kalloc/Verif_basic_allocation.v
@@ -1,0 +1,147 @@
+Require Import VST.floyd.proofauto.
+
+Require Import VC.ASI_kalloc.
+Require Import VC.kallocfun.
+Require Import VC.Spec_kalloc.
+Require Import VC.clientsfun.
+Require Import VC.tactics.
+
+Require Import VC.kalloc.
+
+
+
+Local Open Scope logic.
+
+
+Definition kalloc_write_42_spec : ident * funspec :=
+    DECLARE _kalloc_write_42
+    WITH sh : share, original_freelist_pointer:val, xx:Z, ls:list val, gv:globals
+    PRE [ ] 
+        PROP () PARAMS() GLOBALS(gv) SEP (KF_globals gv sh ls xx original_freelist_pointer)
+    POST [ tint ] 
+        EX r,
+        PROP ( ) RETURN (r) SEP (
+            (if eq_dec original_freelist_pointer nullval then
+                (!! (r = Vint (Int.repr 0)) &&
+                KF_globals gv  sh ls xx original_freelist_pointer * emp)
+            else
+            EX next ls',
+                (!! (next :: ls' = ls /\
+                    r = Vint (Int.repr 42)
+                 ) &&
+                    data_at sh tint (Vint (Int.repr 42)) original_freelist_pointer *
+                    KF_globals gv  sh ls' xx next
+            )
+            )
+        ).
+
+Definition kalloc_int_array_spec : ident * funspec :=
+    DECLARE _kalloc_int_array
+    WITH sh : share, original_freelist_pointer:val, xx:Z, ls:list val, gv:globals, n:Z
+    PRE [ tint ] 
+    PROP (0 <= n <= PGSIZE) PARAMS(Vint (Int.repr n)) GLOBALS(gv) SEP (KF_globals gv sh ls xx original_freelist_pointer)
+    POST [ tptr tint ]
+    PROP ( ) RETURN () SEP (
+        (if eq_dec original_freelist_pointer nullval then
+            KF_globals gv  sh ls xx original_freelist_pointer * emp
+        else
+        EX next ls',
+            (!! (next :: ls' = ls) &&
+                array_42_rep sh n original_freelist_pointer*
+                KF_globals gv  sh ls' xx next
+        )
+        )
+    ).
+
+Lemma body_kalloc_write_42: semax_body KFVprog KFGprog f_kalloc_write_42 kalloc_write_42_spec.
+Proof.
+start_function.
+forward. 
+forward_call (kalloc_spec_sub KF_APD tint) (gv, sh , ls, xx, original_freelist_pointer ). (* kalloc *)
+- unfold KF_globals. entailer!.
+- if_tac.
+    + forward_if.
+        * rewrite H in H0; auto_contradict.
+        * forward. Exists (Vint(Int.repr 0)). entailer.
+    + Intros ab.
+      destruct ls; auto_contradict.
+      forward_if.
+        * unfold type_kalloc_token. rewrite kalloc_token_sz_split. Intros.
+        rewrite memory_block_data_at_; auto. rewrite data_at__eq. forward.
+        forward. forward.
+        Exists (Vint(Int.repr 42)) (fst ab) (snd ab). entailer.
+        * forward.
+Qed.
+
+
+Lemma body_kalloc_int_array: semax_body KFVprog KFGprog f_kalloc_int_array kalloc_int_array_spec.
+Proof.
+start_function.
+forward.
+forward_call (kalloc_spec_sub KF_APD (tarray tint n)) (gv, sh , ls, xx, original_freelist_pointer ). (* kalloc *)
+- unfold KF_globals. entailer!.
+- if_tac.
+    + forward_if.
+        * rewrite H0 in H1; auto_contradict.
+        * forward. 
+    + Intros ab.
+      destruct ls; auto_contradict.
+      forward_if.
+        * unfold type_kalloc_token. rewrite kalloc_token_sz_split. Intros.
+        rewrite memory_block_data_at_; auto. rewrite data_at__eq.
+        forward_for_simple_bound n
+        (EX i:Z,
+        PROP  ()
+        LOCAL (
+            temp _pa original_freelist_pointer; gvars gv;
+            temp _n (Vint (Int.repr n))
+            ) 
+        SEP (
+            (
+                tmp_array_42_rep sh n original_freelist_pointer i*
+                KF_globals gv sh ls xx v
+            )
+            )
+        )%assert.
+        -- apply Z.le_trans with (m:= PGSIZE); try rep_lia. unfold PGSIZE; try rep_lia.
+        -- entailer!. unfold tmp_array_42_rep. unfold KF_globals. entailer!. inversion H1; entailer.
+        -- Intros.
+        assert (Int.min_signed <= i <= Int.max_signed). { 
+            split; try rep_lia. apply Z.le_trans with (m:= n); try rep_lia.
+            apply Z.le_trans with (m:= PGSIZE); try rep_lia. unfold PGSIZE; try rep_lia.
+        } unfold tmp_array_42_rep.
+        forward. entailer.
+        unfold tmp_array_42_rep. entailer!. 
+        rewrite upd_Znth_unfold.
+        ++ rewrite sublist_firstn. 
+        rewrite firstn_app1.
+        assert (Zlength (array_42 (Z.to_nat i)) = i). { rewrite array_42_length. try rep_lia. }
+        rewrite Zlength_length in H13; try rep_lia.
+        rewrite <- H13 at 1.
+        rewrite firstn_exact_length with (xs :=array_42 (Z.to_nat i)); try rep_lia.
+        rewrite sublist_app2.
+        rewrite array_42_length.
+        replace (i + 1 - Z.of_nat (Z.to_nat i)) with (1); try rep_lia.
+        rewrite Zlength_app.
+        rewrite array_42_length.
+        replace (Z.of_nat (Z.to_nat i) + Zlength (Zrepeat (default_val tint) (n - i)) -
+        Z.of_nat (Z.to_nat i)) with (Zlength (Zrepeat (default_val tint) (n - i))); try rep_lia.
+        rewrite Zlength_Zrepeat; try rep_lia.
+        rewrite sublist_Zrepeat; try rep_lia.
+        replace (Z.to_nat (i + 1)) with (Z.to_nat (i) + 1)%nat; try rep_lia.
+        rewrite <- array_42_append.
+        replace (n - i - 1) with (n - (i + 1)); try rep_lia. 
+        rewrite app_assoc. entailer!.
+        ** rewrite array_42_length. try rep_lia.
+        ** assert (Datatypes.length (array_42 (Z.to_nat i))%nat = Z.to_nat i). {
+            rewrite <- Zlength_length; try rep_lia.
+            rewrite array_42_length.
+            try rep_lia.
+        }
+        rewrite H13; auto.
+        ++ rewrite Zlength_app. rewrite array_42_length. rewrite Zlength_Zrepeat; try rep_lia.
+        -- forward. Exists v ls. entailer!. unfold tmp_array_42_rep. unfold array_42_rep. 
+        replace (n - n) with 0; try rep_lia. 
+        rewrite Zrepeat_0. rewrite app_nil_r. entailer!.
+    * forward.
+Qed.
