kalloc/Verif_kfree_loops.v
@@ -1,0 +1,346 @@
+Require Import VST.floyd.proofauto.
+
+Require Import VC.ASI_kalloc.
+Require Import VC.kallocfun.
+Require Import VC.Spec_kalloc.
+Require Import VC.clientsfun.
+Require Import VC.tactics.
+
+Require Import VC.kalloc.
+
+
+
+Local Open Scope logic.
+
+Definition kfree_kfree_kalloc_loop_spec := 
+    DECLARE _kfree_kfree_kalloc_loop
+    WITH sh : share, pa1:val, original_freelist_pointer:val, xx:Z, gv:globals, ls : list val, next:val
+    PRE [ tptr tvoid ]
+        PROP(
+            isptr pa1 /\ (* just assume it is pointers for simplicity *)
+            Int.min_signed <= Int.signed (Int.repr 2) + Int.signed (Int.repr 1) <= Int.max_signed
+        ) 
+        PARAMS (pa1) GLOBALS(gv)
+        SEP (
+            kalloc_tokens Tok_APD sh (2)%nat pa1 PGSIZE t_run *
+            KF_globals gv sh ls xx original_freelist_pointer
+        )
+    POST [ tptr tvoid ]
+        PROP( )
+            RETURN (offset_val PGSIZE pa1) (* we return the head like in the pop function*)
+            SEP 
+            (
+                (*data_at sh t_run pa1 (offset_val PGSIZE pa1) **)
+                kalloc_token' KF_APD sh (sizeof t_run) (offset_val PGSIZE pa1) *
+                KF_globals gv sh (original_freelist_pointer::ls) xx pa1
+                ).
+
+Definition kfree_loop_spec := 
+    DECLARE _kfree_loop
+    WITH sh : share, pa1:val, original_freelist_pointer:val, xx:Z, gv:globals, ls : list val, n:Z
+    PRE [ tptr tvoid, tint ]
+        PROP(
+            isptr pa1 /\
+            Int.min_signed <= Int.signed (Int.repr n) + Int.signed (Int.repr 1) <= Int.max_signed /\
+            0 <= n <= Int.max_signed
+        ) 
+        PARAMS (pa1; Vint (Int.repr n)) GLOBALS(gv)
+        SEP (
+            kalloc_tokens Tok_APD sh (Z.to_nat n)%nat pa1 PGSIZE t_run *
+            KF_globals gv sh ls xx original_freelist_pointer
+        )
+    POST [ tvoid ]
+        EX head, EX added_elem, (* TODO: fix top and next is the same?? *)
+        PROP( 
+            added_elem = (pointers_with_original_head (Z.to_nat n) (pa1) PGSIZE original_freelist_pointer) /\
+            head = (hd nullval ((pointers_with_original_head (Z.to_nat n+1) (pa1) PGSIZE original_freelist_pointer)++ls))
+            )
+            RETURN () (* we return the head like in the pop function*)
+            SEP 
+            (
+                KF_globals gv sh (added_elem++ls) xx head
+            ).
+
+Definition kfree_loop_kalloc_spec := 
+    DECLARE _kfree_loop_kalloc
+    WITH sh : share, pa1:val, original_freelist_pointer:val, xx:Z, gv:globals, ls : list val, n:Z
+    PRE [ tptr tvoid, tint ]
+        PROP(
+            isptr pa1 /\
+            Int.min_signed <= Int.signed (Int.repr n) + Int.signed (Int.repr 1) <= Int.max_signed /\
+            0 <= n <= Int.max_signed
+        ) 
+        PARAMS (pa1; Vint (Int.repr n)) GLOBALS(gv)
+        SEP (
+            kalloc_tokens Tok_APD sh (Z.to_nat n)%nat pa1 PGSIZE t_run *
+            KF_globals gv sh ls xx original_freelist_pointer
+        )
+    POST [ tptr tvoid ]
+        EX head, EX added_elem, (* TODO: fix top and next is the same?? *)
+        PROP( 
+            (* before alloc *)
+            added_elem = (pointers_with_original_head (Z.to_nat n) (pa1) PGSIZE original_freelist_pointer) /\
+            head = (hd nullval ((pointers_with_original_head (Z.to_nat n+1) (pa1) PGSIZE original_freelist_pointer)++ls))
+            )
+            RETURN (head) (* we return the head like in the pop function*)
+            SEP 
+            (
+            let n_eq_0_case :=
+                if eq_dec original_freelist_pointer nullval then
+                emp * KF_globals gv sh ls xx original_freelist_pointer
+            else
+                EX next, EX ls',
+                    !! (next :: ls' = ls) &&
+                    KF_globals gv sh ls' xx next *
+                    kalloc_token' KF_APD sh (sizeof t_run) original_freelist_pointer
+            in
+            let n_gt_0_case :=
+                KF_globals gv sh ((tl added_elem)++ls) xx (hd nullval added_elem) *
+                kalloc_token' KF_APD sh (sizeof t_run) head
+            in
+            if (Z.ltb 0 n) then
+                n_gt_0_case
+            else 
+                n_eq_0_case
+                ).
+
+
+Definition KFGprog_clients: funspecs := KFGprog ++ [kfree_loop_spec].
+
+
+Lemma body_kfree_kfree_kalloc_loop: semax_body  KFVprog KFGprog f_kfree_kfree_kalloc_loop kfree_kfree_kalloc_loop_spec.
+Proof.
+    start_function.
+    Intros. forward. (*forward. unfold abb iate in POSTCONDITION.*)
+    forward_while 
+    (EX i:Z, EX p_tmp:val, EX curr_head:val, EX tmp_added_elem : list val,
+    PROP  (
+        0 <= i <= 2 /\
+        ((curr_head = original_freelist_pointer /\ i = 0) \/ (curr_head = (offset_val (-PGSIZE) (p_tmp))  /\ i <> 0)) /\
+        tmp_added_elem = (pointers_with_original_head (Z.to_nat i) (pa1) PGSIZE original_freelist_pointer) /\
+        p_tmp = offset_val (i * PGSIZE)%Z pa1 /\
+        Int.min_signed <=
+        Int.signed (Int.repr i) + Int.signed (Int.repr 1) <=
+        Int.max_signed 
+    )
+    LOCAL (
+        gvars gv;
+        temp _pa_start p_tmp;
+        temp _i (Vint (Int.repr i))
+        ) 
+    SEP (
+        (
+        KF_globals gv sh (tmp_added_elem ++ ls) xx curr_head *
+        kalloc_tokens Tok_APD sh (Z.to_nat(2-i)) p_tmp (PGSIZE) t_run
+        )
+        )
+    )%assert; destruct H as [H H3].
+    - entailer. Exists 0 pa1 original_freelist_pointer (pointers_with_original_head (Z.to_nat 0) pa1 PGSIZE original_freelist_pointer). (*entailer. *)
+        rewrite <- pointers_with_head_empty. simpl; entailer!; unfold offset_val in H2; destruct pa1; auto_contradict.
+    - entailer.
+    - Intros. destruct (Z.to_nat (2 - i)) eqn:e.
+        +assert (i = 2); try rep_lia.
+        + forward_call (kfree_spec_sub KF_APD t_run) (p_tmp, gv, sh , (tmp_added_elem ++ ls), xx,curr_head). (* call kfree*)
+            * if_tac; destruct H0 as [H01 [H02 [H03 [H04 H05]]]]; rewrite H04 in H1.
+                -- unfold offset_val in H1. destruct pa1; auto_contradict.
+                --unfold KF_globals. unfold type_kalloc_token. rewrite kalloc_token_sz_split. simpl. rewrite kalloc_token_sz_split. Intros.
+                entailer!.
+            * destruct H0 as [H01 [H02 [H03 [H04 H05]]]]; rewrite H04. unfold is_pointer_or_null.
+              unfold offset_val. destruct pa1; auto_contradict; auto.
+            * forward. entailer!. destruct H0 as [H01 [H02 [H03 [H04 H05]]]]; rewrite H04. unfold is_pointer_or_null.
+            unfold offset_val. destruct pa1; auto_contradict; auto.
+            forward. if_tac; auto_contradict; destruct H0 as [H01 [H02 [H03 [H04 H05]]]]; rewrite H04 in H1.
+                -- unfold offset_val in H1. destruct pa1; auto_contradict.
+                -- Exists ((((i+1)%Z, (offset_val PGSIZE p_tmp):val), p_tmp:val), (curr_head::(pointers_with_original_head(Z.to_nat (i)) pa1 PGSIZE)original_freelist_pointer):list val).
+                entailer!. 
+                ++ split; try rep_lia. split.
+                    ** right. split; try rep_lia. replace (i * PGSIZE + PGSIZE + - PGSIZE) with (i * PGSIZE)%Z; try rep_lia.
+                    auto.
+                    ** split.
+                        --- destruct H02 as [[H0211 H0212] | [H0221 H0222]].
+                            +++ rewrite H0212. simpl. rewrite H0211. auto.
+                            +++ rewrite sub_add_offset_n in H0221; auto; try rep_lia.
+                            2: {
+                            unfold PGSIZE; try rep_lia.
+                            }
+                            rewrite H0221.
+                            replace (i - 1) with (Z.of_nat ((Z.to_nat i) - 1)%nat); try rep_lia.
+                            replace (Z.to_nat (i + 1)) with (((Z.to_nat i) + 1)%nat); try rep_lia.
+                            rewrite add_to_pointers_with_head; auto; try rep_lia.
+                        --- replace (i * PGSIZE + PGSIZE) with ((i + 1) * PGSIZE)%Z; try rep_lia; auto.
+                ++ unfold KF_globals. 
+                assert (Z.to_nat (2 - (i + 1)) = n); try rep_lia.
+                rewrite H6. rewrite app_comm_cons. entailer!.
+    - forward_call (kalloc_spec_sub KF_APD t_run) (gv, sh , pa1::original_freelist_pointer::ls, xx, offset_val PGSIZE pa1). (* kalloc *)
+        +
+        (*- forward_call (sh, add_offset pa1 PGSIZE, xx, (pa1::original_freelist_pointer::ls), gv). (* call kalloc *)*)
+        entailer. destruct H0 as [H01 [H02 [H03 [H04 H05]]]]; rewrite H04 in H1.
+        unfold KF_globals. rewrite H03.
+        rewrite mem_mgr_split.
+         
+        assert (i = 2); try rep_lia. rewrite H0. destruct (0 <? Z.to_nat 2)%nat eqn:ei; try rep_lia.
+        * destruct H02 as [[H021 H022] | [H031 H032]]; try rep_lia.
+          rewrite H04 in H031. rewrite sub_add_offset_n in H031; auto; try rep_lia.
+          Intros.
+          destruct (Z.to_nat 2) eqn:e2; auto_contradict.
+          unfold pointers_with_original_head.
+          destruct n eqn:en; try rep_lia.
+          destruct n0 eqn:en0; try rep_lia.
+          simpl. rewrite mem_mgr_split. refold_freelistrep. entailer!.
+          unfold PGSIZE; rep_lia.
+        * rewrite Nat.ltb_ge in ei. try rep_lia.
+        + destruct H0 as [H01 [H02 [H03 [H04 H05]]]].
+        forward. if_tac.
+        assert (isptr (offset_val PGSIZE pa1)). {
+            apply isptr_offset_val'; auto.
+        }
+        rewrite H1 in H2; auto_contradict.
+        Intros ab. unfold type_kalloc_token, KF_globals. 
+        inversion H2. entailer!.
+Qed.
+
+
+Lemma body_kfree_loop: semax_body KFVprog KFGprog f_kfree_loop kfree_loop_spec.
+Proof.
+start_function.
+Intros. forward. (*forward. unfold abb iate in POSTCONDITION.*)
+    forward_while 
+    (EX i:Z, EX p_tmp:val, EX curr_head:val, EX tmp_added_elem : list val,
+    PROP  (
+        0 <= i <= n /\
+        ((curr_head = original_freelist_pointer /\ i = 0) \/ (curr_head = (offset_val (-PGSIZE) (p_tmp))  /\ i <> 0)) /\
+        tmp_added_elem = (pointers_with_original_head (Z.to_nat i) (pa1) PGSIZE original_freelist_pointer) /\
+        p_tmp = offset_val (i * PGSIZE)%Z pa1 /\
+        Int.min_signed <=
+        Int.signed (Int.repr i) + Int.signed (Int.repr 1) <=
+        Int.max_signed 
+    )
+    LOCAL (
+        gvars gv;
+        temp _pa_start p_tmp;
+        temp _i (Vint (Int.repr i));
+        temp _n (Vint (Int.repr n))
+        ) 
+    SEP (
+        (
+            KF_globals gv sh (tmp_added_elem ++ ls) xx curr_head *
+            kalloc_tokens Tok_APD sh (Z.to_nat(n-i)) p_tmp (PGSIZE) t_run
+        )
+    ))%assert; destruct H as [H01 [H02 H03]].
+    - entailer. Exists 0 pa1 original_freelist_pointer (pointers_with_original_head (Z.to_nat 0) pa1 PGSIZE original_freelist_pointer). (*entailer. *)
+        rewrite <- pointers_with_head_empty. entailer. destruct (Z.to_nat n).
+            + rewrite <- H0 in H01. try rep_lia.
+            + rewrite app_nil_l. entailer!.
+    - entailer.
+    - Intros. destruct (Z.to_nat (n - i)) eqn:e1.
+        + try rep_lia.
+        + forward_call (kfree_spec_sub KF_APD t_run) (p_tmp, gv, sh , (tmp_added_elem ++ ls), xx,curr_head). (* call kfree*)
+        (*forward_call (sh, p_tmp, curr_head, xx, gv, (tmp_added_elem ++ ls), PGSIZE). (* call kfree1 *)*)
+            *if_tac; destruct H0 as [H001 [H002 [H003 [H04 H05]]]]. rewrite H04 in H.
+            -- unfold offset_val in H. destruct pa1; auto_contradict.
+            --unfold KF_globals. unfold type_kalloc_token. rewrite kalloc_token_sz_split. simpl. rewrite kalloc_token_sz_split. Intros.
+            entailer!.
+            * destruct H0 as [H001 [H002 [H003 [H04 H05]]]]. rewrite H04.
+                assert ( isptr (offset_val (i * PGSIZE) pa1)). {apply isptr_offset_val'. auto. }
+                auto.
+            * forward. 
+                --entailer!. destruct H0 as [H001 [H002 [H003 [H04 H05]]]]. rewrite H04.
+                assert ( isptr (offset_val (i * PGSIZE) pa1)). {apply isptr_offset_val'. auto. }
+                auto.
+                -- forward. if_tac_auto_contradict.
+                ++ destruct H0 as [H001 [H002 [H003 [H04 H05]]]]. rewrite H04.
+                assert ( isptr (p_tmp)). { rewrite H04. apply isptr_offset_val'. auto. }
+                rewrite H in H0; auto_contradict.
+                ++ Exists ((((i+1)%Z, (offset_val PGSIZE p_tmp):val), p_tmp:val), ((pointers_with_original_head(Z.to_nat (i+1)) pa1 PGSIZE)original_freelist_pointer):list val).
+                entailer!; destruct H0 as [H001 [H002 [H003 [H04 H05]]]].
+                    **simpl. do 2 split; try rep_lia. split. 
+                        --- right. split. rewrite isptr_offset_val_zero; auto.
+                        rewrite H04. apply isptr_offset_val'. auto.
+                        destruct H002 as [[H0021 H0022] | [H0021 H0022]]; try rep_lia.
+                        --- split.
+                        destruct (Z.to_nat i) eqn:ei.
+                        destruct H002 as [[H0021 H0022] | [H0021 H0022]]; try rep_lia.
+                        rewrite H04. rewrite H0022. unfold PGSIZE; auto. simpl. rewrite isptr_offset_val_zero; auto.
+                         rewrite <- add_add_offset_n; auto; try rep_lia.
+                         rewrite H04. auto.
+                         unfold PGSIZE; rep_lia.
+                        assert (n + 1 <= Int.max_signed); try rep_lia.
+                        rewrite Int.signed_repr in H02; try rep_lia. rewrite Int.signed_repr in H02; try rep_lia.
+                        --- rewrite sem_add_pi'; auto. rewrite H04. apply isptr_offset_val'. auto.
+                        try rep_lia.
+                    ** unfold KF_globals.
+                    
+
+                    assert (Z.to_nat (n - (i + 1)) = n0); try rep_lia.
+                    rewrite H0.
+                    assert (curr_head :: tmp_added_elem = pointers_with_original_head (Z.to_nat (i + 1)) pa1 PGSIZE original_freelist_pointer). {
+                        rewrite H003.
+                        destruct H002 as [[H0021 H0022] | [H0021 H0022]].
+                        - rewrite H0022. simpl. rewrite H0021. auto.
+                        - replace (Z.to_nat (i + 1)) with (((Z.to_nat i) + 1)%nat); try rep_lia.
+                        rewrite <- add_to_pointers_with_head; auto.
+                        rewrite H0021; rewrite H04.
+                        rewrite sub_add_offset_n; auto; try rep_lia.
+                        replace (Z.of_nat (Z.to_nat i - 1))%Z with ((i - 1))%Z; try rep_lia.
+                        auto.
+                        unfold PGSIZE; rep_lia.
+                        try rep_lia.
+                    }
+                    rewrite app_comm_cons.
+                    rewrite H5. entailer!.
+    - forward.  Exists curr_head tmp_added_elem. entailer.
+    destruct H0 as [H001 [H002 [H003 [H04 H05]]]].
+    destruct (Z.to_nat (n - i)) eqn:eni; try rep_lia.
+    simpl. entailer!.
+    split. assert (i = n); try rep_lia. rewrite H2. auto.
+    destruct (Z.to_nat n) eqn:en; destruct H002 as [[H0021 H0022] | [H0021 H0022]]; try rep_lia.
+    + simpl. auto.
+    + rewrite <- add_to_pointers_with_head; auto; try rep_lia. simpl.
+    rewrite H0021.  rewrite sub_add_offset_n; auto; try rep_lia.
+    replace (Z.of_nat (n0 - 0)) with (i -1); try rep_lia. auto.
+    unfold PGSIZE; rep_lia.
+Qed.
+
+
+Lemma body_kfree_loop_kalloc: semax_body KFVprog KFGprog_clients f_kfree_loop_kalloc kfree_loop_kalloc_spec.
+Proof.
+start_function.
+forward_call (sh, pa1:val, original_freelist_pointer:val, xx:Z, gv:globals, ls : list val, n:Z).
+- destruct H as [H1 [H2 H3]]; auto.
+- Intros vret. 
+forward_call (kalloc_spec_sub KF_APD t_run) (gv, sh , snd vret ++ ls, xx,  fst vret ); (* kalloc *)
+destruct H as [H11 [H12 H13]]; auto.
+    + unfold KF_globals. entailer!.
+    + if_tac; auto_contradict.
+        * forward. destruct (Z.to_nat n) eqn:en.
+            -- assert (n = 0); try rep_lia. rewrite H3. Exists (fst vret) (snd vret).
+                    entailer.
+                    if_tac_auto_contradict;
+                    destruct (0 <? 0) eqn:efalse; try rep_lia.
+                ++simpl in H0. rewrite H0. simpl in H1. rewrite H1. unfold KF_globals. rewrite app_nil_l. entailer!.
+                ++simpl in H1. rewrite <- H1 in H3. rewrite H in H3; auto_contradict.
+            -- rewrite <- add_to_pointers_with_head in H1; auto; try rep_lia. simpl in H1.
+            assert (isptr (offset_val (Z.of_nat (n0 - 0) * PGSIZE) pa1)). { apply isptr_offset_val'. auto. }
+            rewrite <- H1 in H3. rewrite H in H3; auto_contradict.
+        * forward. destruct (Z.to_nat n) eqn:en.
+            -- Exists (fst vret) (snd vret).
+                assert (n = 0); try rep_lia. rewrite H4.
+                if_tac_auto_contradict;
+                destruct (0 <? 0) eqn:efalse; try rep_lia.
+                ++ unfold KF_globals. entailer!.
+                ++ destruct ls eqn:els.
+                    **  simpl in H0. rewrite H0 in H3. inversion H3.
+                    ** simpl in H1. simpl in H0. Exists (fst ab) (snd ab). unfold KF_globals. rewrite H1.
+                    entailer!. rewrite H0 in H3. rewrite app_nil_l in H3. auto.
+                    unfold type_kalloc_token. entailer!.
+            -- Exists (fst vret) (snd vret).
+                entailer.
+                destruct (0 <? n) eqn:etrue; try rep_lia.
+                unfold KF_globals. unfold type_kalloc_token. entailer!.
+                destruct (snd vret).
+                ++ replace (S n0) with (n0 + 1)%nat in H0; try rep_lia. 
+                destruct n0 eqn:en0.
+                ** simpl in H0. inversion H0.
+                ** rewrite  <- add_to_pointers_with_head in H0; auto; try rep_lia. inversion H0.
+                ++ simpl. rewrite <- app_comm_cons in H3. inversion H3. entailer.
+Qed.
